test/global_array_tactic/helpers/Helper.fst
@@ -5,17 +5,6 @@ let is_sorted (xs: list Int32.t) =
   forall (i j: nat). i < j /\ j < List.length xs ==>
     Int32.v (List.Tot.index xs i) <= Int32.v (List.Tot.index xs j)
 
-assume val array_spec_to_list #a (s: full_array_spec a) : list a
-assume val array_spec_to_list_len #a s : Lemma (List.length (array_spec_to_list #a s) == array_spec_len s) [SMTPat (List.length (array_spec_to_list #a s))]
-assume val array_spec_to_list_idx #a (s: full_array_spec a) (i: nat) :
-  Lemma
-    (requires i < array_spec_len s)
-    (ensures List.Tot.index (array_spec_to_list s) i == array_spec_idx s i)
-    [SMTPat (List.Tot.index (array_spec_to_list s) i)]
-assume val array_spec_to_list_of_list #a (xs: list a) :
-  Lemma (array_spec_to_list (array_spec_of_list xs) == xs)
-    [SMTPat (array_spec_to_list (array_spec_of_list xs))]
-
 let is_sorted_array_spec_to_list_of_list #xs (h: is_sorted xs) :
   is_sorted (array_spec_to_list (array_spec_of_list xs)) = ()
 
